Many things about substitution

HoTTModel/DTT/PTS.lean
@@ -42,7 +42,7 @@ notation N" ↑ "i => lift i 0 N
 
 variable {M N : PTerm S}
 
-lemma lift_inj {i c : ℕ} :
+def lift_inj {i c : ℕ} :
     (M ↑ i # c) = (N ↑ i # c) → M = N := by
   intro h
   induction M generalizing N c with
@@ -82,33 +82,34 @@ lemma lift_inj {i c : ℕ} :
       split_ifs at h
       simpa using ⟨ih₁ h.1, ih₂ h.2⟩
 
-lemma lift0_inj {i : ℕ} :
+def lift0_inj {i : ℕ} :
     (M ↑ i) = (N ↑ i) → M = N :=
   lift_inj
 
-lemma lift_zero {c : ℕ} :
+def lift_zero {c : ℕ} :
     (M ↑ 0 # c) = M := by
   induction M generalizing c
   all_goals simp
   all_goals rename_i ih₁ ih₂
   all_goals exact ⟨ih₁, ih₂⟩
 
-lemma lift_lift (i j k : ℕ) :
+def lift_lift (i j k : ℕ) :
     ((M ↑ j # i) ↑ k # (j + i)) = M ↑ (j + k) # i := by
   sorry
 
-lemma lift_lift_of_le (i j k n : ℕ) :
+def lift_lift_of_le (i j k n : ℕ) :
     i ≤ n → ((M ↑ j # i) ↑ k # (j + n)) = (M ↑ k # n) ↑ j # i := by
   sorry
 
-lemma lift_lift_of_le_of_le (i j k n : ℕ) :
+def lift_lift_of_le_of_le (i j k n : ℕ) :
     i ≤ n → k ≤ i + n → ((M ↑ n # i) ↑ j # k) = M ↑ (n + j) # i := by
   sorry
 
-lemma lift0_lift0 (i j : ℕ) :
+def lift0_lift0 (i j : ℕ) :
     ((M ↑ i) ↑ j) = M ↑ (i + j) :=
   lift_lift_of_le_of_le _ _ _ _ (by simp) (by simp)
 
+@[simp]
 def subst (e : PTerm S) (m : ℕ) : PTerm S → PTerm S
 | #n => if n < m then #n else (if n = m then e ↑ n else #(n - 1))
 | sort M => !M
@@ -120,25 +121,25 @@ notation N "{" e " // " m "}" => subst e m N
 
 notation N "{" e "}" => subst e 0 N
 
-lemma subst_lift (i j k : ℕ) :
+def subst_lift (i j k : ℕ) :
     (M{N // j} ↑ k # (j + i)) = (M ↑ k # j + i + 1){N ↑ k # i // j} := by
   sorry
 
-lemma subst_lift_of_le (i j n : ℕ) :
+def subst_lift_of_le (i j n : ℕ) :
     i ≤ n → (M{N // n} ↑ j # i) = (M ↑ j # i){N // j + n} := by
   sorry
 
-lemma lift_subst_of_le_of_le (i j k : ℕ) :
+def lift_subst_of_le_of_le (i j k : ℕ) :
     i ≤ k → k ≤ i + n → (M ↑ (n + 1) # j){N // k} = M ↑ n # i := by
   sorry
 
 variable {P : PTerm S}
 
-lemma subst_subst (i j : ℕ) :
+def subst_subst (i j : ℕ) :
     M{N // j}{P // i + j} = M{P // i + j + 1}{N{P // i} // j} := by
   sorry
 
-lemma subst0_subst0 (k : ℕ) :
+def subst0_subst0 (k : ℕ) :
     M{N}{P // k} = M{P // k + 1}{N{P // k}} :=
   subst_subst _ 0
 
@@ -148,6 +149,8 @@ section Context
 
 def PCtx (S : Specification) := List (PTerm S)
 
+abbrev PCtx.lift (i c : ℕ) : PCtx S → PCtx S := List.map (PureTypeSystem.lift i c)
+
 variable {α : Type*}
 
 inductive isItem : α → List α → ℕ → Prop
@@ -156,9 +159,13 @@ inductive isItem : α → List α → ℕ → Prop
 
 notation x " ↓ " n " in " Γ => isItem x Γ n
 
+lemma isItem.lt_length : ∀ (_ : x ↓ n in Γ), n < length Γ
+| .zero _ => by simp
+| .succ x h => by simp; apply lt_length h
+
 -- need a better name
 
-lemma isItem_unique {x y : α} {Γ : List α} {n : ℕ} :
+def isItem_unique {x y : α} {Γ : List α} {n : ℕ} :
     (x ↓ n in Γ) → (y ↓ n in Γ) → x = y := by
   induction n generalizing x y Γ
   . intro h₁ h₂
@@ -169,11 +176,24 @@ lemma isItem_unique {x y : α} {Γ : List α} {n : ℕ} :
     apply ih h₁ h₂
 
 -- isTruncate the first k-term and have =
-inductive isTrunc : ℕ → List α → List α → Prop
+inductive isTrunc : ℕ → List α → List α → Type _
 | zero Γ : isTrunc 0 Γ Γ
 | succ {k : ℕ} {Γ Γ' : List α} (x : α) : isTrunc k Γ Γ' → isTrunc (k + 1) (x :: Γ) Γ'
 
-lemma exist_isTrunc_of_isItem (k : ℕ) (Γ : List α) (x : α) :
+def isTrunc.pred : ∀ {k Γ Δ} {A : PTerm S} (_ : isTrunc k Γ (A :: Δ)), isTrunc (k + 1) Γ Δ
+| 0, _, _, _, h => by cases h; apply isTrunc.succ; apply isTrunc.zero
+| k, [], Δ, A, h => by cases h
+| k + 1, B :: Γ, Δ, A, h => by
+    apply isTrunc.succ
+    cases h
+    apply isTrunc.pred (by assumption)
+
+def isTrunc.nil_length {Γ : List α}: ∀ {k} (_ : isTrunc k Γ []), Γ.length = k
+| 0, h => by cases h; rfl
+| k + 1, .succ x h => by simp only [length_cons, nil_length h]
+
+/-
+def exist_isTrunc_of_isItem (k : ℕ) (Γ : List α) (x : α) :
     (x ↓ k in Γ) → ∃ Γ', isTrunc (k + 1) Γ Γ' := by
   induction k generalizing x Γ
   . intro h; cases h; rename_i Γ
@@ -182,12 +202,17 @@ lemma exist_isTrunc_of_isItem (k : ℕ) (Γ : List α) (x : α) :
     rename_i ih _ _ h
     obtain ⟨Γ', hΓ'⟩ := ih _ _ h
     exact ⟨Γ', isTrunc.succ _ hΓ'⟩
+-/
+def isIerm_of_isTrunc {Γ Δ : List α} {A : α} : ∀ {k : ℕ},
+    isTrunc k Γ (A :: Δ) → A ↓ k in Γ
+| 0, h => by cases h; apply isItem.zero
+| k + 1, .succ _ h => isItem.succ _ (isIerm_of_isTrunc h)
 
-inductive isInsert (Γ : PCtx S) (t : PTerm S) : ℕ → PCtx S → PCtx S → Prop
+inductive isInsert (Γ : PCtx S) (t : PTerm S) : ℕ → PCtx S → PCtx S → Type _
 | zero : isInsert Γ t 0 Γ (t :: Γ)
 | succ {n Δ Δ'} u : isInsert Γ t n Δ Δ' → isInsert Γ t (n + 1) (u :: Δ) ((u ↑ 1 # n) :: Δ')
 
-lemma isItem_of_isInsert_of_le {t : PTerm S} {n : ℕ} {Γ Δ Δ' : PCtx S} :
+def isItem_of_isInsert_of_le {t : PTerm S} {n : ℕ} {Γ Δ Δ' : PCtx S} :
     isInsert Γ t n Δ Δ' → ∀ {k}, (n ≤ k → ∀ {u}, (u ↓ k in Δ) → u ↓ k + 1 in Δ') := by
   induction n generalizing t Δ Δ'
   . intro h k hk u hu; cases h
@@ -203,7 +228,7 @@ lemma isItem_of_isInsert_of_le {t : PTerm S} {n : ℕ} {Γ Δ Δ' : PCtx S} :
       simp at hk
       apply ih ht hk hu
 
-lemma isItem_of_isInsert_of_lt {t : PTerm S} {n : ℕ} {Γ Δ Δ' : PCtx S} :
+def isItem_of_isInsert_of_lt {t : PTerm S} {n : ℕ} {Γ Δ Δ' : PCtx S} :
     isInsert Γ t n Δ Δ' → ∀ {k}, (k < n → ∀ {u}, (u ↓ k in Δ) →
       (u ↑ 1 # (n - (k + 1)) ) ↓ k in Δ') := by
   sorry
@@ -213,10 +238,9 @@ def isItemLift (t : PTerm S) (Γ : PCtx S) (n : ℕ) : Prop :=
 
 notation x " ↓ " n " sub " Γ => isItemLift x Γ n
 
-lemma isItemLift_of_isInsert_of_lt {t : PTerm S} {n : ℕ} {Γ Δ Δ' : PCtx S} :
-    isInsert Γ t n Δ Δ' → ∀ {k}, (k < n → ∀ {u}, (u ↓ k sub Δ) →
-      (u ↑ 1 # n) ↓ k sub Δ') := by
-  intro h k hk u hu
+def isItemLift_of_isInsert_of_lt {t u : PTerm S} {n : ℕ} {Γ Δ Δ' : PCtx S}
+  (h : isInsert Γ t n Δ Δ') {k : ℕ} (hk : k < n) (hu : u ↓ k sub Δ) :
+    (u ↑ 1 # n) ↓ k sub Δ' := by
   rcases hu with ⟨w, ⟨hw₁, hw₂⟩⟩
   use w ↑ 1 # (n - (k + 1))
   constructor
@@ -235,11 +259,11 @@ lemma isItemLift_of_isInsert_of_lt {t : PTerm S} {n : ℕ} {Γ Δ Δ' : PCtx S} 
         simp at hk ⊢
         apply isItem_of_isInsert_of_lt ht hk hw
 
-inductive isSubst (Γ : PCtx S) (t T : PTerm S) : ℕ → PCtx S → PCtx S → Prop
+inductive isSubst (Γ : PCtx S) (t T : PTerm S) : ℕ → PCtx S → PCtx S → Type _
 | zero : isSubst Γ t T 0 (T :: Γ) Γ
 | succ {n Δ Δ'} w : isSubst Γ t T n Δ Δ' → isSubst Γ t T (n + 1) (w :: Δ) (w{t // n} :: Δ')
 
-lemma isTerm_of_isSubst_of_le {n : ℕ} {Γ Δ Δ' : PCtx S} {t T : PTerm S} :
+def isTerm_of_isSubst_of_le {n : ℕ} {Γ Δ Δ' : PCtx S} {t T : PTerm S} :
     isSubst Γ t T n Δ Δ' → ∀ {k}, n ≤ k → (∀ {v}, (v ↓ k + 1 in Δ) → v ↓ k in Δ') := by
   induction n
   . intro h k hk v hv
@@ -253,7 +277,7 @@ section Reduction
 
 variable {S : Specification}
 
-inductive beta : PTerm S → PTerm S → Prop
+inductive beta : PTerm S → PTerm S → Type _
 | head (A M N : PTerm S) : beta ((λ.A M) ⬝ N) (M{N ↑ 1 # 0 // 0})
 | appl (A A' M : PTerm S) : beta A A' → beta (A ⬝ M) (A' ⬝ M)
 | appr (A M M' : PTerm S) : beta M M' → beta (A ⬝ M) (A ⬝ M')
@@ -262,287 +286,738 @@ inductive beta : PTerm S → PTerm S → Prop
 | absl (A A' M : PTerm S) : beta A A' → beta (λ.A M) (λ.A' M)
 | absr (A M M' : PTerm S) : beta M M' → beta (λ.A M) (λ.A M')
 
-open Relation
-
-def betar := ReflTransGen (@beta S)
-
-def betac := EqvGen (@beta S)
-
 infix:50 " →β " => beta
+
+inductive betar : PTerm S → PTerm S → Type _
+| beta x y : x →β y → betar x y
+| refl x : betar x x
+| trans x y z : betar x y → betar y z → betar x z
+
 infix:50 " ↠β " => betar
+
+inductive betac : PTerm S → PTerm S → Type _
+| betar x y : x ↠β y → betac x y
+| symm x y : betac x y → betac y x
+| trans x y z : betac x y → betac y z → betac x z
+
 infix:50 " ≃β " => betac
+
+def betac.refl (A : PTerm S) : A ≃β A := betac.betar _ _ (betar.refl _)
+
+def lift_beta_lift (h : A →β B) :
+    (A ↑ i # n) →β B ↑ i # n := by
+  sorry
+
+def lift_betac_lift (h : A ≃β B) :
+    (A ↑ i # n) ≃β B ↑ i # n := by
+  sorry
 
 end Reduction
 
 section Typing
 
-inductive PJudge (S : Specification)
-| wf : PCtx S → PJudge S
-| typing : PCtx S → PTerm S → PTerm S → PJudge S
+mutual
+inductive wf {S : Specification} : PCtx S → Type _
+| nil : wf []
+| cons Γ A s : typing Γ A (!s) → wf (A :: Γ)
 
-open PJudge Relation
+inductive typing {S : Specification} : PCtx S → PTerm S → PTerm S → Type _
+| var Γ A n : wf Γ → (A ↓ n sub Γ) → typing Γ (#n) A
+| sort Γ s₁ s₂ (h : S.ax s₁ s₂) : wf Γ → typing Γ (!s₁) (!s₂)
+| pi Γ A B s₁ s₂ s₃ (h : S.rel s₁ s₂ s₃) :
+    typing Γ A (!s₁) →  typing (A :: Γ) B (!s₂) → typing Γ (Π.A B) (!s₃)
+| abs Γ A b B s₁ s₂ s₃ (h : S.rel s₁ s₂ s₃) :
+    typing Γ A (!s₁) →  typing (A :: Γ) B (!s₂) → typing (A :: Γ) b B →
+      typing Γ (λ.A b) (Π.A B)
+| app Γ f A B a :
+    typing Γ f (Π.A B) → typing Γ a A → typing Γ (f ⬝ a) (B{a})
+| conv Γ a A B s (h : A ≃β B):
+    typing Γ a A → typing Γ B (!s) → typing Γ a B
 
-notation (priority := high) "⬝" => ([] : PCtx _)
+end
+
+#check typing.rec
 notation:20 Γ " ⊢ ⬝ " => wf Γ
 notation:20 Γ " ⊢ " a  " : " A => typing Γ a A
 
-inductive Derivable {S : Specification} : PJudge S → Prop
-| nil : Derivable ((⬝ : PCtx S) ⊢ ⬝)
-| cons Γ A s : Derivable (Γ ⊢ A : !s) → Derivable (A :: Γ ⊢ ⬝)
-| var Γ A n : Derivable (Γ ⊢ ⬝) → (A ↓ n sub Γ) → Derivable (Γ ⊢ #n : A)
-| sort Γ s₁ s₂ (h : S.ax s₁ s₂) : Derivable (Γ ⊢ ⬝) → Derivable (Γ ⊢ !s₁ : !s₂)
-| pi Γ A B s₁ s₂ s₃ (h : S.rel s₁ s₂ s₃) :
-    Derivable (Γ ⊢ A : !s₁) →  Derivable (A :: Γ ⊢ B : !s₂) → Derivable (Γ ⊢ Π.A B : !s₃)
-| abs Γ A b B s₁ s₂ s₃ (h : S.rel s₁ s₂ s₃) :
-    Derivable (Γ ⊢ A : !s₁) →  Derivable (A :: Γ ⊢ B : !s₂) → Derivable (A :: Γ ⊢ b : B) →
-      Derivable (Γ ⊢ λ.A b : Π.A B)
-| app Γ f A B a :
-    Derivable (Γ ⊢ f : Π.A B) → Derivable (Γ ⊢ a : A) → Derivable (Γ ⊢ f ⬝ a : B{a})
-| conv Γ a A B s (h : A ≃β B):
-    Derivable (Γ ⊢ a : A) → Derivable (Γ ⊢ B : !s) → Derivable (Γ ⊢ a : B)
-
 variable {S : Specification}
 
-lemma cons_inv (h : Derivable (A :: Γ ⊢ ⬝)) :
-    ∃ s, Derivable (Γ ⊢ A : !s) := by
+def wf_of_typing : ∀ (_ : Γ ⊢ t : T), Γ ⊢ ⬝
+| .var _ _ _ _ _ => by assumption
+| .sort _ _ _ _ _ => by assumption
+| .pi _ _ _ _ _ _ _ h _ => wf_of_typing h
+| .abs _ _ _ _ _ _ _ _ h _ _ => wf_of_typing h
+| .app _ _ _ _ _ h _ => wf_of_typing h
+| .conv Γ a A B s h₀ h₁ h₂ => wf_of_typing h₁
+
+lemma exists_of_cons (h : A :: Γ ⊢ ⬝) : ∃ s, Nonempty (Γ ⊢ A : !s) := by
   cases h with
-  | cons _ _ s h => exact ⟨s, h⟩
+  | cons Γ A s h => exact ⟨s, ⟨h⟩⟩
 
-lemma exists_of_var_typing (h : Derivable (Γ ⊢ #n : A)) :
-    ∃ B, B ≃β A ∧ (B ↓ n sub Γ) := by
-  generalize hJ : (Γ ⊢ #n : A) = J at h
-  induction h generalizing A
-  all_goals cases hJ
-  . rename_i A _ _ _
-    exact ⟨A ,⟨EqvGen.refl _, by assumption⟩⟩
-  . rename_i h₁ _ _ _ h₂
-    obtain ⟨C, hC⟩ := h₂ rfl
-    exact ⟨C, ⟨EqvGen.trans _ _ _ hC.1 h₁, hC.2⟩⟩
+def exists_of_cons' (h : A :: Γ ⊢ ⬝) : Σs, (Γ ⊢ A : !s) := by
+  cases h with
+  | cons Γ A s h => exact ⟨s, h⟩
 
-lemma exists_of_sort_typing (h : Derivable (Γ ⊢ !s : A)) :
-    ∃ t, ((!t) ≃β A) ∧ S.ax s t := by
-  generalize hJ : (Γ ⊢ !s : A) = J at h
-  induction h generalizing A
+def wf_of_cons (h : A :: Γ ⊢ ⬝) : Γ ⊢ ⬝ :=
+  wf_of_typing (exists_of_cons' h).snd
+
+open Relation
+/-
+lemma exists_of_var_typing : ∀ (_ : Γ ⊢ #n : A),
+    ∃ B, B ≃β A ∧ (B ↓ n sub Γ)
+| .var _ _ _ h₀ h₁ => ⟨A ,⟨EqvGen.refl _, by assumption⟩⟩
+| .conv _ _ B _ s h₀ h₁ h₂ => by
+    obtain ⟨C, hC⟩ := exists_of_var_typing h₁
+    use C
+    exact ⟨EqvGen.trans _ _ _ hC.1 h₀, hC.2⟩
+
+def exists_of_sort_typing : ∀ (_ : Γ ⊢ !s : A),
+    ∃ t, ((!t) ≃β A) ∧ S.ax s t
+| .sort _ _ t h₀ h₁ => ⟨t, ⟨EqvGen.refl _, by assumption⟩⟩
+| .conv _ _ B _ s h₀ h₁ h₂ => by
+    obtain ⟨C, hC⟩ := exists_of_sort_typing h₁
+    use C
+    exact ⟨EqvGen.trans _ _ _ hC.1 h₀, hC.2⟩
+-/
+/-
+def exists_of_pi_typing : ∀ (_ : Γ ⊢ Π.A B : T),
+    ∃ s₁ s₂ s₃, (T ≃β !s₃) ∧ S.rel s₁ s₂ s₃ ∧ Nonempty (Γ ⊢ A : !s₁) ∧ Nonempty (A :: Γ ⊢ B : !s₂) :=
+  sorry
+
+def exists_of_abs_typing (h : Derivable (Γ ⊢ λ.A b : T)) :
+    ∃ s₁ s₂ s₃, ∃ B, (T ≃β Π.A B) ∧ S.rel s₁ s₂ s₃ ∧
+      Derivable (Γ ⊢ A : !s₁) ∧ Derivable (A :: Γ ⊢ b : B) ∧
+      Derivable (A :: Γ ⊢ B : !s₂) := by
+  generalize hJ : (Γ ⊢ λ.A b : T) = J at h
+  induction h generalizing A b T
   all_goals cases hJ
-  . rename_i A _ _ _
-    exact ⟨A ,⟨EqvGen.refl _, by assumption⟩⟩
-  . rename_i h₁ _ _ _ h₂
-    obtain ⟨t, ht⟩ := h₂ rfl
-    exact ⟨t, ⟨EqvGen.trans _ _ _ ht.1 h₁, ht.2⟩⟩
+  . rename_i B s₁ s₂ s₃ _ _ _ _ _ _ _
+    use s₁, s₂, s₃, B
+    exact ⟨EqvGen.refl _, ⟨by assumption, ⟨by assumption, ⟨by assumption, by assumption⟩⟩⟩⟩
+  . rename_i h _ _ _ ih
+    obtain ⟨s₁, ⟨s₂, ⟨s₃, ⟨B, hs⟩⟩⟩⟩ := ih rfl
+    use s₁, s₂, s₃, B
+    exact ⟨EqvGen.trans _ _ _ (EqvGen.symm _ _ h) hs.1, hs.2⟩
+
+def exists_of_app_typing (h : Derivable (Γ ⊢ f ⬝ a : T)) :
+    ∃ A B, T ≃β B{a} ∧ Derivable (Γ ⊢ f : Π.A B) ∧ Derivable (Γ ⊢ a : A) := by
+  generalize hJ : (Γ ⊢ f ⬝ a : T) = J at h
+  induction h generalizing f a T
+  all_goals cases hJ
+  . rename_i A B _ _ _ _ _
+    use A, B
+    exact ⟨EqvGen.refl _, ⟨by assumption, by assumption⟩⟩
+  . rename_i h _ _ _ ih
+    obtain ⟨A, ⟨B, h'⟩⟩ := ih rfl
+    use A, B
+    exact ⟨EqvGen.trans _ _ _ (EqvGen.symm _ _ h) h'.1, h'.2⟩
+-/
+
+mutual
+def weakening_typing : ∀ (_ : Γ ⊢ t : T) (_ : isInsert Δ A n Γ Γ') (_ : Δ ⊢ A : !s),
+    (Γ' ⊢ t ↑ 1 # n : T ↑ 1 # n)
+| .var Γ A k h₀ h₁, h₂, h₃ => by
+  dsimp
+  split_ifs with h
+  . apply typing.var _ _ _ _
+      (isItemLift_of_isInsert_of_lt h₂ h h₁)
+    apply (weakening_wf h₀ h₂ h₃)
+  . apply typing.var _ _ _ (weakening_wf h₀ h₂ h₃)
+    obtain ⟨T', hT'⟩ := h₁
+    use T'
+    rw [hT'.1]
+    constructor
+    . rw [lift_lift_of_le_of_le _ _ _ _ (by simp)
+        (by simp at h ⊢; apply h.trans (Nat.le_succ _))]
+    . apply isItem_of_isInsert_of_le h₂ (by simpa using h) hT'.2
+| .sort Γ s₁ s₂ h₀ h₁, h₂, h₃ => by
+    simp; apply typing.sort _ _ _ h₀ (weakening_wf h₁ h₂ h₃)
+| .pi Γ A B s₁ s₂ s₃ h₀ h₁ h₃, h₄, h₅ => by
+  apply typing.pi
+  apply h₀
+  apply weakening_typing h₁ h₄ h₅
+  apply weakening_typing h₃ (h₄.succ A) h₅
+| .abs Γ A b B s₁ s₂ s₃ h₀ h₁ h₂ h₃, h₄, h₅ => by
+  apply typing.abs
+  apply h₀
+  apply weakening_typing h₁ h₄ h₅
+  apply weakening_typing h₂ (h₄.succ A) h₅
+  apply weakening_typing h₃ (h₄.succ A) h₅
+| .app Γ f A B a h₀ h₁, h₂, h₃ => by
+  have : n = 0 + n := by simp
+  rw [this, subst_lift]; simp
+  apply typing.app
+  apply weakening_typing h₀ h₂ h₃
+  apply weakening_typing h₁ h₂ h₃
+| .conv Γ a A B s h₀ h₁ h₂, h₃, h₄ => by
+  apply typing.conv _ _ (A ↑ 1 # n) _ _ (lift_betac_lift h₀)
+  apply weakening_typing h₁ h₃ h₄
+  apply weakening_typing h₂ h₃ h₄
+
+def weakening_wf : ∀ (_ : Γ ⊢ ⬝) (_ : isInsert Δ A n Γ Γ') (_ : Δ ⊢ A : !s),
+    (Γ' ⊢ ⬝)
+| _, .zero, h₃ => wf.cons _ _ _ h₃
+| _, .succ u (Δ := Γ) (n := n) h₂, h₃ => by
+    rename_i h₁ _
+    cases h₁
+    rename_i s h₀
+    apply wf.cons _ _ s
+    have : (!s) = ((!s) ↑ 1 # n) := by rfl
+    rw [this]
+    apply weakening_typing h₀ h₂ h₃
+end
+
+#check ℕ
+
+def lift_inv_of_typing : ∀ (_ : Γ ⊢ t : T), (t ↑ 1 # Γ.length) = t
+| .var Γ T n h₁ ⟨B, h₂⟩ => by simp [h₂.2.lt_length]
+| .sort _ _ _ _ _ => by simp
+| .conv _ _ _ _ _ _ h _ => lift_inv_of_typing h
+| .app _ _ _ _ _ h₁ h₂ => by
+  simp; exact ⟨lift_inv_of_typing h₁, lift_inv_of_typing h₂⟩
+| .abs _ _ _ _ _ _ _ _ h₀ _ h₂ => by
+  simp; exact ⟨lift_inv_of_typing h₀, lift_inv_of_typing h₂⟩
+| .pi _ _ _ _ _ _ _ h₀ h₁ => by
+  simp; exact ⟨lift_inv_of_typing h₀, lift_inv_of_typing h₁⟩
+
+def lift_inv_of_typing'  (h : Γ ⊢ t : T) : (T ↑ 1 # Γ.length) = T := sorry
+
+def lift_inv_of_typing''  (h : T :: Γ ⊢ ⬝) : (T ↑ 1 # Γ.length) = T := sorry
+
+def isInsert_length : ∀ {Γ Δ : PCtx S} (_ : Δ ⊢ ⬝ ),
+  isInsert Γ A (length Δ) (List.append Δ Γ) (List.append Δ (A :: Γ))
+| Γ, [], h => by simp; apply isInsert.zero
+| Γ, B :: Δ, h => by
+  simp
+  convert isInsert.succ _ _
+  rw [lift_inv_of_typing'' h]
+  apply isInsert_length (wf_of_cons h)
+
+def append_typing : ∀ {Γ Δ : PCtx S} (_ : Γ ⊢ ⬝) (_ : Δ ⊢ t : T),
+    List.append Δ Γ ⊢ t : T
+| [], Δ, h₁, h₂ => by simpa
+| A :: Γ, Δ, wf.cons _ _ s h₁, h₂ => by
+  simp
+  rw [← lift_inv_of_typing h₂, ← lift_inv_of_typing' h₂]
+  apply weakening_typing (append_typing (wf_of_typing h₁) h₂) _ h₁
+  apply isInsert_length (wf_of_typing h₂)
+
+def append_wf : ∀ {Γ Δ : PCtx S} (_ : Γ ⊢ ⬝) (_ : Δ ⊢ ⬝), List.append Δ Γ ⊢ ⬝
+| _, [], h, _ => h
+| Γ, A :: Δ, h₁, .cons _ _ _ h₂ =>
+  weakening_wf (append_wf h₁ (wf_of_typing h₂)) isInsert.zero
+    (append_typing h₁ h₂)
+
+def substitution_typing : ∀ (_ : Γ ⊢ t : T) (_ : isSubst Δ a A n Γ Γ') (_ : Δ ⊢ a : A),
+  Γ' ⊢ t{a//n} : T{a//n} := sorry
+
+def substitution_wf : ∀ (_ : Γ ⊢ ⬝ ) (_ : isSubst Δ a A n Γ Γ') (_ : Δ ⊢ a : A),
+  Γ' ⊢ ⬝ := sorry
 
 end Typing
 
-
-/-
-section Typing
+section beta
 
 open Relation
+variable {S : Specification}
 
-notation (priority := high) "⬝" => ([] : PCtx _)
+namespace PCtx
 
-mutual
+inductive beta : PCtx S → PCtx S → Type _
+| head {A B Γ} : A →β B → beta (A :: Γ) (B :: Γ)
+| tail {A Γ Δ} : beta Γ Δ → beta (A :: Γ) (A :: Δ)
 
-inductive Wf {S : Specification} : PCtx S → Prop
-| nil : Wf (⬝ : PCtx S)
-| cons Γ A s : Der Γ A (!s) → Wf (A :: Γ)
+infix:50 " →β " => beta
 
-inductive Der {S : Specification} : PCtx S → PTerm S → PTerm S → Prop
-| var Γ A n : Wf Γ → (A ↓ n sub Γ) → Der Γ (#n) A
-| sort Γ s₁ s₂ (h : S.ax s₁ s₂) : Wf Γ → Der Γ (!s₁) (!s₂)
-| pi Γ A B s₁ s₂ s₃ (h : S.rel s₁ s₂ s₃) :
-    Der Γ A (!s₁) →  Der (A :: Γ) B (!s₂) → Der Γ (Π.A B) (!s₃)
-| abs Γ A b B s₁ s₂ s₃ (h : S.rel s₁ s₂ s₃) :
-    Der Γ A (!s₁) →  Der (A :: Γ) B (!s₂) → Der (A :: Γ) b B → Der Γ (λ.A b) (Π.A B)
-| app Γ f A B a :
-    Der Γ f (Π.A B) → Der Γ a A → Der Γ (f ⬝ a) (B{a})
-| conv Γ a A B s (h : A ≃β B):
-    Der Γ a A → Der Γ B (!s) → Der Γ a B
+inductive betar : PCtx S → PCtx S → Type _
+| beta (x y : PCtx S) : x →β y → betar x y
+| refl x : betar x x
+| trans x y z : betar x y → betar y z → betar x z
 
-end
+infix:50 " ↠β " => betar
 
-notation:20 Γ " ⊢ ⬝ " => Wf Γ
-notation:20 Γ " ⊢ " a  " : " A => Der Γ a A
+inductive betac : PCtx S → PCtx S → Type _
+| betar (x y : PCtx S) : x ↠β y → betac x y
+| symm x y : betac x y → betac y x
+| trans x y z : betac x y → betac y z → betac x z
 
+infix:50 " ≃β " => betac
 
-lemma cons_inv (h : (A :: Γ) ⊢ ⬝) :
-    ∃ s, Γ ⊢ A : !s := by
-  cases h with
-  | cons _ _ s h => exact ⟨s, h⟩
+variable {Γ Δ : PCtx S} {A B : PTerm S}
 
-lemma var_inv (h : Γ ⊢ #n : A) :
-    ∃ B, B ≃β A ∧ (B ↓ n sub Γ) := by
-  induction h
-  sorry
+lemma beta.length_eq : ∀ {Γ Δ : PCtx S} (_ : Γ →β Δ), Γ.length = Δ.length
+| A :: Γ, B :: _, .head h => rfl
+| A :: Γ, _ :: Δ, .tail h => by simp [h.length_eq]
 
-end
--/
+lemma betar.length_eq {Γ Δ : PCtx S} : ∀ (_ : Γ ↠β Δ), Γ.length = Δ.length
+| .beta _ _ h => h.length_eq
+| .refl _ => rfl
+| .trans _ _ _ h₁ h₂ => h₁.length_eq.trans h₂.length_eq
+
+lemma betac.length_eq {Γ Δ : PCtx S} : ∀ (_ : Γ ≃β Δ), Γ.length = Δ.length
+| .betar _ _ h => h.length_eq
+| .symm _ _ h => h.length_eq.symm
+| .trans _ _ _ h₁ h₂ => h₁.length_eq.trans h₂.length_eq
+
+lemma betar.nil (h : Γ ↠β []) : Γ = [] := by
+  simpa using h.length_eq
+
+def betar.head {Γ Δ : PCtx S} {A B : PTerm S} : ∀ (_ : (A :: Γ) ↠β (B :: Δ)), A ↠β B
+| .beta _ _ (beta.head h) => PureTypeSystem.betar.beta _ _ h
+| .beta _ _ (beta.tail h) => PureTypeSystem.betar.refl _
+| .refl _ =>  PureTypeSystem.betar.refl _
+| .trans _ [] _ h₁ h₂ => by simpa using h₁.length_eq
+| .trans _ (C :: Θ) _ h₁ h₂ => (head h₁).trans _ _ _ (head h₂)
+
+def betac.head {Γ Δ : PCtx S} {A B : PTerm S} : ∀ (_ : (A :: Γ) ≃β (B :: Δ)), A ≃β B
+| .betar _ _ h => PureTypeSystem.betac.betar _ _ h.head
+| .symm _ _ h => PureTypeSystem.betac.symm _ _ (head h)
+| .trans _ [] _ h₁ h₂ => by simpa using h₁.length_eq
+| .trans _ (C :: Θ) _ h₁ h₂ => (head h₁).trans _ _ _ (head h₂)
+
+end PCtx
+
+def term_betar_typing : ∀ {Γ : PCtx S} {t s M} (_: Γ ⊢ t : M) (_ : t ↠β s), Γ ⊢ s : M := sorry
+
+-- reduced to expansion???
+def term_betac_typing : ∀ {Γ : PCtx S} {t s M} (_: Γ ⊢ t : M) (_ : t ≃β s), Γ ⊢ s : M
+| Γ, t, s, M, h, .betar _ _ h' => term_betar_typing h h'
+| Γ, t, s, M, h, .symm _ _ h' => by sorry
+| Γ, t, s, M, h, .trans _ r _ h₁ h₂ => by sorry
+
+end beta
 
 section Morphism
 
-def SubstSq (t : PTerm S) : ℕ → PCtx S → PTerm S
+@[simp]
+def simulSubst (t : PTerm S) : ℕ → PCtx S → PTerm S
 | _, [] => t
-| n, A :: Γ => (SubstSq t (n + 1) Γ){A // n}
+| n, A :: Γ => (simulSubst t (n + 1) Γ){A // n}
+-- ((simulSubst t (n + 1) Γ) ↑ 1 # (n + 1)){A ↑ 1// n}
 
-example : SubstSq T 0 [] = T := rfl
+@[simp]
+def simulSubstCtx : PCtx S → ℕ → PCtx S → PCtx S
+| [], _, _ => []
+| A :: Γ, n, Δ => simulSubst A (n + Γ.length) Δ :: simulSubstCtx Γ n Δ
 
-example : SubstSq T 0 [f] = T{f // 0} := rfl
+@[simp]
+lemma simulSubstCtx_nil : ∀ {Γ : PCtx S} {n}, simulSubstCtx Γ n [] = Γ
+| [], _ => rfl
+| A :: Γ, _ => by simp only [simulSubstCtx, simulSubst, simulSubstCtx_nil]
 
-example : SubstSq T 0 [g, f] = T{f // 1}{g // 0} := rfl
+lemma simulSubst_sort {s : S.sort} {n : ℕ} : ∀ {Γ : PCtx S},
+    simulSubst (!s) n Γ = (!s : PTerm S)
+| [] => rfl
+| _ :: _ => by dsimp [simulSubst]; rw [simulSubst_sort]; rfl
 
-example : SubstSq T 0 [g, f] = T{f // 1}{g // 0} := rfl
+lemma simulSubst_pi {A B : PTerm S} {n : ℕ} : ∀ {Γ : PCtx S},
+    simulSubst (Π.A B) n Γ = Π. (simulSubst A n Γ) (simulSubst B (n + 1) Γ)
+| [] => rfl
+| C :: Γ => by simp [simulSubst]; rw [simulSubst_pi]; rfl
 
-example : SubstSq T 0 [h, g, f] = T{f // 2}{g // 1}{h // 0} := rfl
+lemma simulSubst_abs {A B : PTerm S} {n : ℕ} : ∀ {Γ : PCtx S},
+    simulSubst (λ.A B) n Γ = λ. (simulSubst A n Γ) (simulSubst B (n + 1) Γ)
+| [] => rfl
+| C :: Γ => by simp [simulSubst]; rw [simulSubst_abs]; rfl
 
-inductive isMor (Γ : PCtx S) : PCtx S → PCtx S → Prop
+lemma simulSubst_app {A B : PTerm S} {n : ℕ} : ∀ {Γ : PCtx S},
+    simulSubst (A ⬝ B) n Γ = (simulSubst A n Γ) ⬝ (simulSubst B n Γ)
+| [] => rfl
+| C :: Γ => by simp [simulSubst]; rw [simulSubst_app]; rfl
+
+lemma simulSubst_append {t : PTerm S} {n : ℕ} : ∀ {Γ Δ : PCtx S},
+    simulSubst t n (List.append Γ Δ) =
+      simulSubst (simulSubst t (n + Γ.length) Δ) n Γ
+| [], _ => rfl
+| A :: Γ, Δ => by
+  simp; erw [simulSubst_append, Nat.add_assoc, Nat.add_comm 1]
+
+inductive isSimulSubst : PCtx S → ℕ → PCtx S → PCtx S → Type _
+| nil Γ n : isSimulSubst Γ n [] Γ
+| cons Γ n f F Γ' Γs Δ A s :
+  isSimulSubst Γ' (n + 1) F Γ → isTrunc (n + 1) Γ Γs →
+  (Γs ⊢ A : !s) → (Γs ⊢ f : A) → -- isInsert Γs A (n + 1) Γ Γ₁ →
+  isSubst Γs f A n Γ Δ → isSimulSubst Γ' n (f :: F) Δ
+
+def simulSubst_wf (h : Γ' ⊢ ⬝) : ∀ (_ : isSimulSubst Γ' n F Γ),
+    Γ ⊢ ⬝
+| .nil Γ n => h
+| .cons Γ n f F Γ' Γs Δ A s h₁ h₂ h₃ h₄ h₅ =>
+  substitution_wf (simulSubst_wf h h₁) h₅ h₄
+
+def simulSubst_typing (h : Γ' ⊢ t : T) : ∀ (_ : isSimulSubst Γ' n F Γ),
+    Γ ⊢ simulSubst t n F : simulSubst T n F
+| .nil Γ n => h
+| .cons Γ n f F Γ' Γs Δ A s h₁ h₂ h₃ h₄ h₅ =>
+  substitution_typing (simulSubst_typing h h₁) h₅ h₄
+
+inductive isMor (Γ : PCtx S) : PCtx S → PCtx S → Type _
 | nil : isMor Γ [] []
-| cons : isMor Γ Δ F → Derivable (Γ ⊢ f : (SubstSq D 0 F)) → isMor Γ (D :: Δ) (f :: F)
+| cons : isMor Γ Δ F → (Γ ⊢ simulSubst D 0 F : !s) →
+    (Γ ⊢ f : (simulSubst D 0 F)) → isMor Γ (D :: Δ) (f :: F)
 
-example (Γ Δ F : PCtx S) :
-    isMor Γ Δ F → Δ.length = F.length := by
-  intro h
-  induction Δ generalizing F with
-  | nil => cases h; rfl
-  | cons A Δ ih =>
-      cases h
-      rename_i h
-      simp [ih _ h]
+lemma isSubst.length_eq_add_one {Γ Δ Δ' : PCtx S} : ∀ (_ : isSubst Γ f A n Δ Δ'),
+  Δ.length = Δ'.length + 1
+| .zero => by simp
+| .succ _ h => by simp; apply length_eq_add_one h
 
-example : isMor [T₁, T₀] [T₁, T₀] [#1, #0] := by
-  apply isMor.cons
-  apply isMor.cons
-  apply isMor.nil
-  . simp [SubstSq]; sorry
-  . simp [SubstSq]; sorry
+lemma isSubst.length_lt {Γ Δ Δ' : PCtx S} (h : isSubst Γ f A n Δ Δ') :
+    Δ'.length < Δ.length := by
+  rw [length_eq_add_one h]
+  simp only [Nat.lt_add_one]
 
-example : isMor [#0, T] [#0, T] [#0, #1] := by
-  apply isMor.cons
-  apply isMor.cons
-  apply isMor.nil
-  . simp [SubstSq]; sorry
-  . simp [SubstSq, subst]
-    apply Derivable.var
-    . sorry
-    . use #0; simp; apply isItem.zero
+lemma isSimulSubst.length_le {Γ F Δ : PCtx S} : ∀ (_ : isSimulSubst Γ n F Δ),
+    Δ.length ≤ Γ.length
+| .nil Γ n => le_refl _
+| .cons Γ n f F Γ' Γs Δ A s h₁ h₂ h₃ h₄ h₅ =>
+  h₅.length_lt.le.trans h₁.length_le
 
-example : isMor [#0, #0, T] [#0, #0, T] [#0, #1, #2] := by
-  apply isMor.cons
-  apply isMor.cons
-  apply isMor.cons
-  apply isMor.nil
-  . simp [SubstSq]; sorry
-  . simp [SubstSq, subst]
-    apply Derivable.var
-    . sorry
-    . use #0; simp; apply isItem.succ; apply isItem.zero
-  . simp [SubstSq, subst]
-    apply Derivable.var
-    . sorry
-    . use #0; simp; apply isItem.zero
+lemma isSimulSubst.nil_of_nil {F Δ : PCtx S} (h : isSimulSubst [] n F Δ) :
+    Δ = [] := by
+  apply List.eq_nil_of_length_eq_zero
+  apply Nat.eq_zero_of_le_zero
+  apply h.length_le
 
-example : isMor [(#0) ⬝ #1, #0, T] [(#0) ⬝ #1, #0, T] [#0, #1, #2] := by
-  apply isMor.cons
-  apply isMor.cons
-  apply isMor.cons
-  apply isMor.nil
-  . simp [SubstSq]; sorry
-  . simp [SubstSq, subst]
-    apply Derivable.var
-    . sorry
-    . use #0; simp; apply isItem.succ; apply isItem.zero
-  . simp [SubstSq, subst]
-    apply Derivable.var
-    . sorry
-    . use (#0) ⬝ #1; simp; apply isItem.zero
+def isSimulSubst.append : ∀ {Γ Θ F} (_ : isSimulSubst Γ k F Θ),
+  isSimulSubst (A :: Γ) (k + 1) F ((simulSubst A k F) :: Θ)
+| Γ, Θ, [], h => by cases h; apply nil
+| Γ, Θ, f :: F, .cons Γ' _ _ _ _ Γs _ C s h₁ h₂ h₃ h₄ h₅ => by
+  simp
+  apply cons
+  apply append h₁
+  apply h₂.succ
+  apply h₃
+  apply h₄
+  apply isSubst.succ _ h₅
 
-def id₀ : ℕ → PCtx S →  PCtx S
+def isSimulSubst.drop : ∀ {Γ Δ F} (_ : isSimulSubst (D :: Γ) (k + 1) F (A :: Δ)),
+  isSimulSubst Γ k F Δ
+| Γ, Δ, [], h => by cases h; apply nil
+| Γ, Δ, f :: F, .cons _ _ _ _ _ _ _ _ _ h₁ (isTrunc.succ _ h₂) h₃ h₄ (isSubst.succ _ h₅) =>
+  cons _ _ _ _ _ _ _ _ _ h₁.drop h₂ h₃ h₄ h₅
+
+def isTrunc.eq : ∀ {Γ Δ Δ' : PCtx S} {k : ℕ}
+  (_ : isTrunc k Γ Δ) (_ : isTrunc k Γ Δ'), Δ = Δ'
+| _, _, _, 0, .zero _, .zero _ => rfl
+| _ :: _, _, _, _ + 1, .succ _ h₁, .succ _ h₂ => h₁.eq h₂
+
+def isSubst.eq : ∀ {Γ Δ Θ Θ' : PCtx S} {f B B' : PTerm S} {k : ℕ}
+  (_ : isSubst Γ f B k Δ Θ) (_ : isSubst Γ f B' k Δ Θ'), Θ = Θ'
+| _, _, _, _, _, _, _, 0, .zero, .zero => rfl
+| _, _, _, _, _, _, _, _ + 1, .succ _ h₁, .succ _ h₂ => by
+  rw [h₁.eq h₂]
+
+def isSimulSubst.eq : ∀ {Γ Δ Δ' F : PCtx S}
+  (_ : isSimulSubst Γ k F Δ) (_ : isSimulSubst Γ k F Δ'), Δ = Δ'
+| Γ, Δ, Δ', [], h₃, h₄ => by cases h₃; cases h₄; rfl
+| Γ, Δ, Δ', f :: F,
+  .cons Γ₀ _ _ _ _ Γs _ B s h₃ h₄ h₅ h₆ h₇,
+  .cons Γ₀' _ _ _ _ Γs' _ B' s' h₃' h₄' h₅' h₆' h₇' => by
+  cases h₃.eq h₃'
+  cases h₄.eq h₄'
+  apply h₇.eq h₇'
+
+abbrev isMor' (Γ Δ F : PCtx S) : Type _ := isSimulSubst (List.append Δ Γ) 0 F Γ
+
+def isMor'_isMor : ∀ {Γ Δ F : PCtx S} (_ : isMor Γ Δ F), isMor' Γ Δ F
+| _, [], _, h => by cases h; apply isSimulSubst.nil
+| _, _, [], h => by cases h; apply isSimulSubst.nil
+| Γ, D :: Δ, f :: F, isMor.cons h₁ h₂ h₃ => by
+  apply isSimulSubst.cons
+  apply isSimulSubst.append (isMor'_isMor h₁)
+  apply isTrunc.succ _ (isTrunc.zero _)
+  have := isMor'_isMor h₁
+  simp [isMor'] at this
+  apply h₂
+  apply h₃
+  apply isSubst.zero
+
+lemma test₂ {Γ Δ F : PCtx S} : ∀ (_ : isSimulSubst Γ n Δ F), Γ.length = Δ.length + F.length
+| .nil _ _ => by simp
+| .cons Γ n f F Γ' Γs Δ A s h₁ h₂ h₃ h₄ h₅ => by
+  rw [test₂ h₁, h₅.length_eq_add_one]
+  simp
+  rw [Nat.add_comm _ 1, ← Nat.add_assoc]
+
+lemma test₄ {Γ Δ : PCtx S} (h : isMor' Γ Δ []) : Δ = [] := by
+  simpa using test₂ h
+
+lemma test₅ {Γ F : PCtx S} (h : isMor' Γ [] F) : F = [] := by
+  simpa using test₂ h
+
+def isMor_isMor' : ∀ {Γ Δ F : PCtx S} (_ : isMor' Γ Δ F), isMor Γ Δ F
+| Γ, [], F, h => by cases test₅ h; apply isMor.nil
+| Γ, Δ, [], h => by cases test₄ h; apply isMor.nil
+| Γ, D :: Δ, f :: F,
+  isSimulSubst.cons _ _ _ _ _ _ _ A s h₁ h₂ h₃ h₄ isSubst.zero  => by
+  rw [(List.cons.inj (h₁.eq h₁.drop.append)).1] at h₃ h₄
+  apply isMor.cons (isMor_isMor' h₁.drop) h₃ h₄
+
+lemma testsimulsubstsubst (i k : ℕ) : ∀ {F : PCtx S},
+    simulSubst T (i + k + 2) F{simulSubst g (i + 1) F // k} =
+      simulSubst (T{g // k}) (i + k + 1) F
+| [] => by simp
+| f :: F => by
+  simp
+  have : i + k + 2 = i + 1 + k + 1 := by
+    rw [Nat.add_assoc, Nat.add_assoc, Nat.add_assoc, Nat.add_left_cancel_iff, Nat.add_comm 1]
+    -- I don't want to import linarith... so
+  rw [this, ← subst_subst (i + 1) k]
+  congr 1
+  rw [Nat.add_assoc, Nat.add_comm 1, ← Nat.add_assoc]
+  apply testsimulsubstsubst
+
+lemma liftaux (hn : k ≤ n ) : ∀ {t : PTerm S} (_ : (t ↑ 1 # k) = t) , t{f//n} = t
+| .var i, h => by simp at h; simp only [subst, if_pos (lt_of_lt_of_le h hn)]
+| .sort _, h => rfl
+| .pi _ _, h => by
+  simp at h ⊢
+  exact ⟨liftaux hn h.1, liftaux (Nat.succ_le_succ hn) h.2⟩
+| .abs _ _, h => by
+  simp at h ⊢
+  exact ⟨liftaux hn h.1, liftaux (Nat.succ_le_succ hn) h.2⟩
+| .app _ _, h => by
+  simp at h ⊢
+  exact ⟨liftaux hn h.1, liftaux hn h.2⟩
+
+lemma liftinv {t: PTerm S} (hn : k ≤ n) : ∀ {F : PCtx S} (_ : (t ↑ 1 # k) = t),
+  simulSubst t n F = t
+| [], _ => by rfl
+| f :: F, h => by
+  simp; rw [liftinv (hn.trans (Nat.le_succ _)) h]
+  apply liftaux hn h
+
+/-
+the following is wrong! k is given by the info of `θ ⊢ T : !s`
+
+lemma testeq {T : PTerm S} : ∀ {F G : PCtx S} ,
+  simulSubst T k (pcomp F G) = simulSubst (simulSubst T k G) k F
+| F, [] => by
+  simp [liftinv]
+  sorry
+| [], g :: G => by
+  simp
+  rw [testeq]
+  rfl
+| f :: F, g :: G => by
+  simp
+  rw [testeq]
+  simp
+  have : k + 1 = 0 + k + 1 := by simp
+  rw [this, ← subst_subst 0 k]
+  simp
+  congr
+  convert testsimulsubstsubst 0 k using 3
+  simp only [Nat.zero_add]
+-/
+
+section pcomp
+
+def pcomp : PCtx S → PCtx S → PCtx S
 | _, [] => []
-| n, _ :: S => (#n) :: (id₀ (n + 1) S)
+| F, g :: G =>  simulSubst g 0 F :: pcomp F G
 
-def id : PCtx S → PCtx S := id₀ 0
+@[simp]
+lemma nil_pcomp : ∀ {G : PCtx S}, pcomp [] G = G
+| [] => rfl
+| g :: G => by simp [pcomp]; rw [nil_pcomp]
 
-example : id [T₃, T₂, T₁, T₀] = [#0, #1, #2, #3] := rfl
+lemma testeq {Γ Δ Θ : PCtx S} {T : PTerm S} (h : Θ' ⊢ T : !s):
+  ∀ {F G : PCtx S} (_ : isMor Γ Δ F) (_ : isMor Δ Θ G) (_ : isTrunc k Θ' Θ),
+  simulSubst T k (pcomp F G) = simulSubst (simulSubst T k G) k F
+| F, [], h₁, h₂, h₃ => by
+  simp
+  cases h₂
+  rw [liftinv (le_refl _)]
+  rw [← h₃.nil_length]
+  apply lift_inv_of_typing h
+| [], G, h₁, h₂, h₃ => by
+  cases h₁
+  simp
+| f :: F, g :: G, h₁, isMor.cons h₂ h₃ h₄, h₅ => by
+  simp
+  rw [testeq h h₁ h₂ (isTrunc.pred h₅)]
+  simp
+  have : k + 1 = 0 + k + 1 := by simp
+  rw [this, ← subst_subst 0 k]
+  simp
+  congr
+  convert testsimulsubstsubst 0 k using 3
+  simp only [Nat.zero_add]
 
-/-
-example (h : Derivable ([] ⊢ A : !s)) : A = A ↑ 1 := by
-  induction A generalizing s
-  . obtain ⟨_, ⟨_, ⟨_, ⟨_, hl⟩⟩⟩⟩ := exists_of_var_typing h
-    cases hl
-  . simp
-  . sorry -- simply exfalso??
-  . rename_i A B ih₁ ih₂
-  . sorry -- similar
+def pcomp_isMor {Γ : PCtx S} : ∀ {Δ Θ F G : PCtx S} (_ : Γ ⊢ ⬝) (_ : Θ ⊢ ⬝)
+    (_ : isMor Γ Δ F) (_ : isMor Δ Θ G),
+  isMor Γ Θ (pcomp F G)
+| Δ, θ, F, [], _, _, h₁, h₂ => by cases h₂; apply isMor.nil
+| Δ, [], F, g :: G, _, _, h₁, h₂ => by cases h₂
+| Δ, T :: Θ , F, g :: G, hΓ, hΘ, h₁, isMor.cons h₂ h₃ h₄ => by
+  apply isMor_isMor'
+  simp [isMor']
+  apply isSimulSubst.cons
+  apply isSimulSubst.append
+  apply isMor'_isMor
+  apply pcomp_isMor hΓ (wf_of_cons hΘ) h₁ h₂
+  apply isTrunc.succ _ (isTrunc.zero _)
+  simpa [simulSubst_sort] using simulSubst_typing (append_typing hΓ h₃) (isMor'_isMor h₁)
+  apply simulSubst_typing (append_typing hΓ h₄) (isMor'_isMor h₁)
+  convert isSubst.zero using 2
+  apply testeq (exists_of_cons' hΘ).snd h₁ h₂ (isTrunc.zero _)
 
-example (h : Derivable (Γ ⊢ A : !s)) : A = A ↑ 1 # Γ.length := by
-  induction A generalizing s
-  . obtain ⟨_, ⟨_, hl⟩⟩ := exists_of_var_typing h
-    cases hl
-  . simp
-  . sorry -- simply exfalso??
-  . rename_i A B ih₁ ih₂
-  . sorry -- similar
--/
+end pcomp
 
-
-example (h : Derivable (A :: Γ ⊢ ⬝ )) : SubstSq A 0 (id₀ 1 Γ) = A ↑ 1 := by
-  induction Γ with
-  | nil =>
-      cases h with
-      | cons _ A s h =>
-          simp [id₀, SubstSq]
-          sorry
-  | cons => sorry
-
-example (Γ : PCtx S) (h : Derivable (Γ ⊢ ⬝)): isMor Γ Γ (id Γ) := by
-  induction Γ with
-  | nil => apply isMor.nil
-  | cons A Γ ih =>
-      apply isMor.cons
-      . sorry
-      . apply Derivable.var
-        assumption
-        use A; constructor
-        . sorry
-        . apply isItem.zero
-
-
-
+section id
 
 
+@[simp]
+def idN : ℕ → ℕ →  PCtx S
+| _, 0 => []
+| n, k + 1 => (#n) :: (idN (n + 1) k)
 
+def id₀ (n : ℕ) (Γ : PCtx S) : PCtx S := idN n Γ.length
 
-end Morphism
+@[simp]
+lemma idN_length {n} : ∀ {k}, (idN n k : PCtx S).length = k
+| 0 => rfl
+| k + 1 => by simp [idN_length]
 
-/-
-inductive isSubstSeq : PCtx S → ℕ → PCtx S → PTerm S → Prop
-| nil : isSubstSeq [T] 0 [] T
-| succ : isSubstSeq (T :: Δ) n [] T → isSubstSeq (S :: (T :: Δ)) (n + 1) [] S
-| cons : isSubstSeq Γ (n + 1) F T' → isSubstSeq Γ n (f :: F) (T'{f // n})
+lemma idN_append_idN : ∀ (n k m : ℕ),
+  List.append (idN n k : PCtx S) (idN (n + k) m) = idN n (k + m)
+| _, 0, _ => by simp
+| n, k + 1, m => by
+  rw [Nat.add_assoc, Nat.add_comm 1 m]; simp
+  rw [Nat.add_comm k 1, ← Nat.add_assoc]
+  apply idN_append_idN
 
-example : isSubstSeq [T] 0 [] T := by
-  apply isSubstSeq.nil
+lemma simulSubst_var_idN_of_lt {n m l : ℕ} (hl : n < l) : ∀ {s : ℕ} ,
+    simulSubst (#n : PTerm S) l (idN m s) = (#n)
+| 0 => rfl
+| s + 1 => by
+  simp; rw [simulSubst_var_idN_of_lt (hl.trans (Nat.lt_succ_self _))]
+  simp [hl]
 
-example : isSubstSeq [T₁, T₀] 0 [f] (T₁{f // 0}) := by
-  apply isSubstSeq.cons
-  apply isSubstSeq.succ
-  apply isSubstSeq.nil
+lemma simulSubst_var_idN_of_length_add_le {n m l : ℕ} : ∀ {s : ℕ} (_ : s + l ≤ n),
+    simulSubst (#n : PTerm S) l (idN m s)  = (#n - s)
+| 0, h => by simp
+| s + 1, h => by
+  simp
+  rw [simulSubst_var_idN_of_length_add_le (by simpa only [Nat.add_comm l, ← Nat.add_assoc])]
+  have : l < n - s := by
+    rw [Nat.lt_sub_iff_add_lt, ← Nat.succ_le_iff]
+    convert h using 1
+    simp [Nat.add_comm l, Nat.add_assoc]
+  simp [if_neg (not_lt_of_lt this), if_neg this.ne.symm, Nat.sub_sub]
 
-example : isSubstSeq [T₂, T₁, T₀] 1 [f] (T₂{f // 1}) := by
-  apply isSubstSeq.cons
-  apply isSubstSeq.succ
-  apply isSubstSeq.succ
-  apply isSubstSeq.nil
+-- can be strengthened???? `n ≤ s`
+lemma simulSubst_var_idN_of_lt_length {n k l : ℕ} {s : ℕ} (hn : n < s) :
+    simulSubst (#n : PTerm S) l (idN k s) = (#n) ↑ k # l := by
+  rcases lt_or_le n l with hl | hl
+  . simp [hl, simulSubst_var_idN_of_lt hl]
+  . obtain ⟨a, ha⟩ := Nat.exists_eq_add_of_le hl
+    have aux₁ : (idN k s : PCtx S) = List.append (idN k a) (idN (k + a) (s - a)) := by
+      convert (idN_append_idN k a (s - a)).symm
+      rw [Nat.add_sub_of_le]
+      apply le_trans _ hn.le
+      simp only [ha, Nat.le_add_left]
+    have aux₂ : idN (k + a) (s - a) = (#k + a : PTerm S) :: (idN (k + a + 1) (s - (a + 1))) := by
+      have : s - a = s - (a + 1) + 1 := by
+        rw [← Nat.sub_add_comm, Nat.add_sub_add_right]
+        apply le_trans _ hn
+        simp [ha]
+      rw [this]; rfl
+    rw [aux₁, aux₂]
+    erw [simulSubst_append] -- no!!
+    simp [if_neg (not_lt_of_le hl)]
+    rw [simulSubst_var_idN_of_lt (by simp only [ha, Nat.lt_add_one])]
+    simp [ha]
+    rw [simulSubst_var_idN_of_length_add_le
+      (by rw [← Nat.add_assoc, Nat.add_assoc k, Nat.add_comm k,
+        Nat.add_assoc]; simp only [Nat.le_add_right])]
+    rw [Nat.add_sub_assoc (by simp), Nat.add_sub_self_right, Nat.add_assoc, Nat.add_comm,
+        Nat.add_comm a]
 
-example : isSubstSeq [T₂, T₁, T₀] 0 [g, f] ((T₂{f // 1}){g // 0}) := by
-  apply isSubstSeq.cons
-  apply isSubstSeq.cons
-  apply isSubstSeq.succ
-  apply isSubstSeq.succ
-  apply isSubstSeq.nil
+lemma simulSubst_var_id₀_of_lt_length {n k l : ℕ} {Γ : PCtx S} (hn : n < Γ.length) :
+    simulSubst (#n) l (id₀ k Γ) = (#n) ↑ k # l :=
+  simulSubst_var_idN_of_lt_length hn
 
-example : isSubstSeq [T'] 0 [] T → T = T' := by
-  intro h; cases h; rfl
+lemma isMorAuxLift' {k l m} : ∀ {A : PTerm S} (_ : (A ↑ 1 # l + m) = A),
+    simulSubst A l (idN k m) = simulSubst A l (idN k (m + 1))
+| .var i, h => by
+    rw [← idN_append_idN k m 1, simulSubst_append]
+    congr
+    have : i < l + m := by simpa using h
+    simp [this]
+| .sort s, _ => by simp [simulSubst_sort]
+| .pi A B, h => by
+    simp only [lift, pi.injEq, simulSubst_pi, subst] at h ⊢
+    refine ⟨isMorAuxLift' h.1, isMorAuxLift' ?_⟩
+    convert h.2 using 1
+    rw [Nat.add_assoc, Nat.add_comm 1, ← Nat.add_assoc]
+| .abs A B, h => by
+    simp only [lift, abs.injEq, simulSubst_abs, subst] at h ⊢
+    refine ⟨isMorAuxLift' h.1, isMorAuxLift' ?_⟩
+    convert h.2 using 1
+    rw [Nat.add_assoc, Nat.add_comm 1, ← Nat.add_assoc]
+| .app A B, h => by
+    simp only [lift, app.injEq, simulSubst_app, subst] at h ⊢
+    refine ⟨isMorAuxLift' h.1, isMorAuxLift' h.2⟩
 
-example : isSubstSeq [T', T''] 0 [] T → False := by
-  intro h
+lemma test2 {k l} (h : k ≤ l) : ∀ {A : PTerm S} (_ : (A ↑ 1 # k) = A), (A ↑ 1 # l) = A
+| .var i, h' => by simp at h' ⊢; apply lt_of_lt_of_le h' h
+| .sort s, _ => rfl
+| .pi _ _, h' => by simp at h' ⊢; exact ⟨test2 h h'.1, test2 (by simpa) h'.2⟩
+| .abs _ _, h' => by simp at h' ⊢; exact ⟨test2 h h'.1, test2 (by simpa) h'.2⟩
+| .app _ _, h' => by simp at h' ⊢; exact ⟨test2 h h'.1, test2 h h'.2⟩
+
+lemma isMorAuxLift {k l m} : ∀ {A : PTerm S} (_ : (A ↑ 1 # m) = A),
+    simulSubst A l (idN k m) = A ↑ k # l
+-- `A` has only var from `0` to `Δ.length - 1`; so `A ↑ Δ.length = A`
+| .var i, h => by
+    rw [simulSubst_var_idN_of_lt_length]
+    simpa using h
+| .sort s, _ => by simp [simulSubst_sort]
+| .pi A B, h => by
+    simp [simulSubst_pi] at h ⊢
+    constructor
+    apply isMorAuxLift h.1
+    rw [isMorAuxLift' (by refine test2 ?_ h.2; rw [Nat.add_assoc, Nat.add_comm 1]; simp)]
+    apply isMorAuxLift h.2
+| .abs A B, h => by
+    simp [simulSubst_abs] at h ⊢
+    constructor
+    apply isMorAuxLift h.1
+    rw [isMorAuxLift' (by refine test2 ?_ h.2; rw [Nat.add_assoc, Nat.add_comm 1]; simp)]
+    apply isMorAuxLift h.2
+| .app A B, h => by
+    simp [simulSubst_app] at h ⊢
+    exact ⟨isMorAuxLift h.1, isMorAuxLift h.2⟩
+
+def aux₁wf (h : A :: Γ ⊢ ⬝) : (A ↑ 1 # Γ.length) = A := by
   cases h
--/
+  apply lift_inv_of_typing (by assumption)
+
+def wf_of_isTrunc {k} {Γ Δ : PCtx S} : ∀ (_ : isTrunc k Γ Δ) (_ : Γ ⊢ ⬝),
+    Δ ⊢ ⬝
+| .zero _, h => h
+| .succ _ _, h => by
+  apply wf_of_isTrunc (by assumption)
+  cases h
+  apply wf_of_typing (by assumption)
+
+
+def isMorAux {k} {Γ Δ : PCtx S} {A} (h₀ : isTrunc k Γ (A :: Δ)) (h₁ : Γ ⊢ ⬝) :
+    Γ ⊢ #k : simulSubst A 0 (id₀ (k + 1) Δ) := by
+  refine typing.var _ _ _ h₁ ⟨A, ⟨?_, isIerm_of_isTrunc h₀⟩⟩
+  apply isMorAuxLift
+  apply aux₁wf
+  apply wf_of_isTrunc h₀ h₁
+
+def id_isMor : ∀ {Γ Δ : PCtx S} (_ : isTrunc k Γ Δ) (_ : Γ ⊢ ⬝), isMor Γ Δ (id₀ k Δ)
+| Γ, [], h, h' => by apply isMor.nil
+| Γ, A :: Δ, h, h' => by
+    apply isMor.cons
+    apply id_isMor (isTrunc.pred h) h'
+    simpa [simulSubst_sort] using simulSubst_typing (append_typing h' (exists_of_cons' (wf_of_isTrunc h h')).snd)
+      (isMor'_isMor (id_isMor (isTrunc.pred h) h'))
+    apply isMorAux h h'
+
+end id
